Add paper version sequential adequacy theorem

src/sequential/SequentialBehavior.v
@@ -227,6 +227,11 @@ Proof.
 Qed.
 
 
+Definition well_formed_state lang (st: lang.(Language.state)): Prop :=
+  forall p m o (WF: Oracle.wf o),
+    SeqBehavior.behavior (@SeqState.na_step _) (SeqThread.mk (SeqState.mk _ st m) p o) <1= SeqBehavior.behavior (@SeqState.na_step_determ _) (SeqThread.mk (SeqState.mk _ st m) p o).
+
+
 Section RECEPTIVE.
   Variable lang: language.
 
